working on casts

deps/poulet4/lib/P4Arith.v
@@ -17,29 +17,32 @@ Module BitArith.
   Section Operations.
     Variable (width : positive).
 
-    Definition upper_bound : Z := 2 ^ Zpos width.
+    Definition upper_bound : Z := 2 ^ pos width.
 
-    Definition maxN : Z := upper_bound - 1.
+    Definition maxZ : Z := upper_bound - 1.
 
     (** Precondition for operations. *)
     Definition bound (n : Z) : Prop := -1 < n < upper_bound.
 
     (* Saturating bound *)
     Definition sat_bound (n : Z) : Z :=
-      if (n >? maxN)
-      then maxN
+      if (n >? maxZ)
+      then maxZ
       else if (n <? 0) then 0 else n.
     (**[]*)
 
     (* Modular bound *)
     Definition mod_bound (n : Z) : Z := n mod upper_bound.
 
+    (* Modular bound with unsigned bit output *)
+    Definition bit_bound := mod_bound.
+
     Lemma upper_bound_ge_1 : 1 <= upper_bound.
     Proof. unfold upper_bound; apply exp_ge_one; lia. Qed.
 
     Lemma sat_bound_bound : forall n, bound (sat_bound n).
     Proof.
-      intros n; unfold sat_bound, bound, maxN.
+      intros n; unfold sat_bound, bound, maxZ.
       destruct (n >? upper_bound -1) eqn:?H.
       - pose proof upper_bound_ge_1. lia.
       - rewrite gtb_ltb in H. rewrite ltb_ge in H.
@@ -145,7 +148,7 @@ Module BitArith.
         arguments are bounded **)
 
     (** Bitwise Not *)
-    Definition bit_not (a : Z) := mod_bound (maxN - a).
+    Definition bit_not (a : Z) := mod_bound (maxZ - a).
 
     (** Bitwise And *)
     Definition bit_and (a b : Z) := mod_bound (land a b).
@@ -160,8 +163,7 @@ Module BitArith.
 
   (** Bitwise concatination of bit with bit/int *)
   Definition concat (w1 w2 : positive) (z1 z2 : Z) : Z :=
-    mod_bound (w1+w2) 
-    (shiftl z1 (pos w2) + (z2 mod (2 ^ pos w2))).
+    mod_bound (w1+w2) (shiftl z1 (pos w2) + (bit_bound w2 z2)).
   (**[]*)
 
 End BitArith.
@@ -220,9 +222,12 @@ Module IntArith.
       if (z >? maxZ)%Z then maxZ
       else if (z <? minZ)%Z then minZ else z.
 
+    (* Modular bound with unsigned bit output *)
+    Definition bit_bound (n : Z) : Z := n mod mod_amt.
+
     (* Modular bound *)
     Definition mod_bound (n : Z) : Z :=
-      let m := n mod mod_amt in
+      let m := bit_bound n in
       if (m <? upper_bound) then m else m - mod_amt.
     (**[]*)
 
@@ -242,7 +247,7 @@ Module IntArith.
 
     Lemma mod_bound_bound: forall z, bound (mod_bound z).
     Proof.
-      intros. unfold mod_bound, bound, minZ, maxZ.
+      intros. unfold mod_bound, bit_bound, bound, minZ, maxZ.
       pose proof (Z_mod_lt z mod_amt mod_amt_gt_0).
       remember (z mod mod_amt) as zz. clear z Heqzz. rename zz into z.
       pose proof upper_bound_ge_1. destruct (z <? upper_bound) eqn: ?H.
@@ -270,7 +275,7 @@ Module IntArith.
 
     Lemma bound_eq: forall z, bound z -> mod_bound z = z.
     Proof.
-      unfold bound, minZ, maxZ. intros. unfold mod_bound. pose proof mod_amt_neq_0.
+      unfold bound, minZ, maxZ. intros. unfold mod_bound, bit_bound. pose proof mod_amt_neq_0.
       destruct (Z_le_gt_dec 0 z).
       - pose proof mod_amt_2_upper_bound.
         assert (z mod mod_amt <? upper_bound = true). {
@@ -309,7 +314,7 @@ Module IntArith.
     Proof.
       intros. pose proof upper_bound_ge_1. pose proof mod_amt_2_upper_bound.
       unfold neg. destruct (eq_dec n minZ).
-      - subst. unfold mod_bound, minZ. rewrite opp_involutive.
+      - subst. unfold mod_bound, bit_bound, minZ. rewrite opp_involutive.
         assert (upper_bound mod mod_amt = upper_bound). { rewrite mod_small; lia. }
         assert (upper_bound mod mod_amt <? upper_bound = false). {
           rewrite ltb_ge. rewrite H2. easy. } rewrite H3. rewrite H2.
@@ -323,7 +328,7 @@ Module IntArith.
         mod_bound (a + mod_bound b) = mod_bound (a + b).
     Proof.
       pose proof mod_amt_neq_0.
-      intros. unfold mod_bound. destruct (b mod mod_amt <? upper_bound) eqn:?H.
+      intros. unfold mod_bound, bit_bound. destruct (b mod mod_amt <? upper_bound) eqn:?H.
       - rewrite add_mod_idemp_r; easy.
       - assert ((a + (b mod mod_amt - mod_amt)) mod mod_amt = (a + b) mod mod_amt). {
           rewrite add_mod; auto. rewrite Zminus_mod_idemp_l.
@@ -376,14 +381,10 @@ Module IntArith.
 
   (** Bitwise concatination of int with int/bit *)
   Definition concat (w1 w2 : positive) (z1 z2 : Z) : Z :=
-    mod_bound (w1+w2) 
-    (shiftl z1 (pos w2) + (z2 mod (2 ^ (pos w2)))). 
-  (**[]*)
+    mod_bound (w1+w2) (shiftl z1 (pos w2) + (bit_bound w2 z2)).
+  (**[]*) 
 
 End IntArith.
-
-
-
 
 (* 
 Compute (IntArith.concat 4 4 (-16) 31).
